new/proof/github_com/goose_lang/goose/testdata/examples/channel_search_replace.v
@@ -1,7 +1,7 @@
 From New.proof Require Export proof_prelude.
 From New.golang.theory Require Import chan.
 From New.proof.github_com.goose_lang.goose.model.channel
-  Require Import protocol.base chan_au_base simple.
+  Require Import idiom.base chan_au_base handoff.
 From New.proof Require Import sync strings time tok_set.
 From New.generatedproof.github_com.goose_lang.goose.testdata.examples Require Import channel.
 
@@ -9,7 +9,7 @@ Section proof.
 Context `{hG: heapGS Σ, !ffi_semantics _ _}.
 Context `{!globalsGS Σ} {go_ctx : GoContext}.
 Context `{!syncG Σ}.
-Context `{!chan_protocolG Σ slice.t}.
+Context `{!chan_idiomG Σ slice.t}.
 Context `{!waitgroup_joinG Σ}.
 
 #[global] Instance : IsPkgInit chan_spec_raw_examples := define_is_pkg_init True%I.
@@ -35,15 +35,15 @@ Definition chanP wg (x y: w64) (s: slice.t) : iProp Σ :=
 
 Definition waitgroupN := nroot .@ "waitgroup".
 
-Lemma wp_worker (γs: simple_names) (ch: loc) (wg: loc) (x y: w64) :
+Lemma wp_worker (γs: handoff_names) (ch: loc) (wg: loc) (x y: w64) :
   {{{ is_pkg_init chan_spec_raw_examples ∗
-      "#Hchan" ∷ is_simple γs ch (chanP wg x y) }}}
+      "#Hchan" ∷ is_chan_handoff γs ch (chanP wg x y) }}}
     @! chan_spec_raw_examples.worker #ch #wg #x #y
   {{{ RET #(); True }}}.
 Proof.
   wp_start. iNamed "Hpre".
   wp_auto.
-  wp_apply (wp_simple_receive with "[$Hchan]").
+  wp_apply (wp_handoff_receive with "[$Hchan]").
   iIntros (s) "Hrcv".
   wp_auto. iPersist "y x".
   iAssert (∃ s,
@@ -69,7 +69,7 @@ Proof.
     { rewrite take_ge; last word. rewrite drop_ge; last word.
       rewrite app_nil_r. iFrame. }
     wp_for_post.
-    wp_apply (wp_simple_receive with "[$Hchan]").
+    wp_apply (wp_handoff_receive with "[$Hchan]").
     iIntros (s') "Hrcv".
     wp_auto. iFrame.
   - rewrite decide_True //. wp_auto.
@@ -113,7 +113,7 @@ Lemma wp_SearchReplace (s: slice.t) (xs: list w64) (x y: w64) :
   }}}
     @! chan_spec_raw_examples.SearchReplace #s #x #y
   {{{ RET #(); s ↦* (search_replace x y xs) }}}.
-Proof using chan_protocolG0 waitgroup_joinG0 syncG0.
+Proof using chan_idiomG0 waitgroup_joinG0 syncG0.
   (* The first overflow:
      implementation adds 1000 at a time, potentially surpassing the slice length
      before clamping. If it goes negative, then the clamping doesn't work. This
@@ -139,7 +139,7 @@ Proof using chan_protocolG0 waitgroup_joinG0 syncG0.
   iIntros (ch γch_names) "(#His_chan & Hcap & Hoc)". simpl. wp_auto.
   iMod (init_WaitGroup with "wg") as (?) "H".
   iMod (join.init with "H") as "Hwg".
-  iMod (start_simple_buffered _ _ (chanP wg_ptr x y) with "[$His_chan] [$Hoc]") as (γch) "#Hchan".
+  iMod (start_handoff_buffered _ _ (chanP wg_ptr x y) with "[$His_chan] [$Hoc]") as (γch) "#Hchan".
   iAssert (∃ (i : w64), "i" ∷ i_ptr ↦ i)%I with "[$i]" as "HH".
   wp_for. iNamed "HH". wp_auto.
   wp_if_destruct.
@@ -191,7 +191,7 @@ Proof using chan_protocolG0 waitgroup_joinG0 syncG0.
   iDestruct (own_slice_split nextOffset with "Hs") as "[Hsection Hs]".
   { subst nextOffset. word. }
   rewrite drop_drop.
-  wp_apply (wp_simple_send with "[Hdone Hsection]").
+  wp_apply (wp_handoff_send with "[Hdone Hsection]").
   { iFrame "#". iDestruct "Hchan" as "[%H' Hsimp]". iSplitL "Hsimp". { iFrame "#". }
     iFrame.
     }
